\batchmode
\documentclass{book}
\RequirePackage{ifthen}




\usepackage[spanish]{babel}
\usepackage{graphics}%
\providecommand{\R}{ \mbox{$I \hspace{-1.3mm} R$} } 




\usepackage[dvips]{color}


\pagecolor[gray]{.7}

\usepackage[latin1]{inputenc}



\makeatletter

\makeatletter
\count@=\the\catcode`\_ \catcode`\_=8 
\newenvironment{tex2html_wrap}{}{}%
\catcode`\<=12\catcode`\_=\count@
\newcommand{\providedcommand}[1]{\expandafter\providecommand\csname #1\endcsname}%
\newcommand{\renewedcommand}[1]{\expandafter\providecommand\csname #1\endcsname{}%
  \expandafter\renewcommand\csname #1\endcsname}%
\newcommand{\newedenvironment}[1]{\newenvironment{#1}{}{}\renewenvironment{#1}}%
\let\newedcommand\renewedcommand
\let\renewedenvironment\newedenvironment
\makeatother
\let\mathon=$
\let\mathoff=$
\ifx\AtBeginDocument\undefined \newcommand{\AtBeginDocument}[1]{}\fi
\newbox\sizebox
\setlength{\hoffset}{0pt}\setlength{\voffset}{0pt}
\addtolength{\textheight}{\footskip}\setlength{\footskip}{0pt}
\addtolength{\textheight}{\topmargin}\setlength{\topmargin}{0pt}
\addtolength{\textheight}{\headheight}\setlength{\headheight}{0pt}
\addtolength{\textheight}{\headsep}\setlength{\headsep}{0pt}
\setlength{\textwidth}{349pt}
\newwrite\lthtmlwrite
\makeatletter
\let\realnormalsize=\normalsize
\global\topskip=2sp
\def\preveqno{}\let\real@float=\@float \let\realend@float=\end@float
\def\@float{\let\@savefreelist\@freelist\real@float}
\def\liih@math{\ifmmode$\else\bad@math\fi}
\def\end@float{\realend@float\global\let\@freelist\@savefreelist}
\let\real@dbflt=\@dbflt \let\end@dblfloat=\end@float
\let\@largefloatcheck=\relax
\let\if@boxedmulticols=\iftrue
\def\@dbflt{\let\@savefreelist\@freelist\real@dbflt}
\def\adjustnormalsize{\def\normalsize{\mathsurround=0pt \realnormalsize
 \parindent=0pt\abovedisplayskip=0pt\belowdisplayskip=0pt}%
 \def\phantompar{\csname par\endcsname}\normalsize}%
\def\lthtmltypeout#1{{\let\protect\string \immediate\write\lthtmlwrite{#1}}}%
\newcommand\lthtmlhboxmathA{\adjustnormalsize\setbox\sizebox=\hbox\bgroup\kern.05em }%
\newcommand\lthtmlhboxmathB{\adjustnormalsize\setbox\sizebox=\hbox to\hsize\bgroup\hfill }%
\newcommand\lthtmlvboxmathA{\adjustnormalsize\setbox\sizebox=\vbox\bgroup %
 \let\ifinner=\iffalse \let\)\liih@math }%
\newcommand\lthtmlboxmathZ{\@next\next\@currlist{}{\def\next{\voidb@x}}%
 \expandafter\box\next\egroup}%
\newcommand\lthtmlmathtype[1]{\gdef\lthtmlmathenv{#1}}%
\newcommand\lthtmllogmath{\lthtmltypeout{l2hSize %
:\lthtmlmathenv:\the\ht\sizebox::\the\dp\sizebox::\the\wd\sizebox.\preveqno}}%
\newcommand\lthtmlfigureA[1]{\let\@savefreelist\@freelist
       \lthtmlmathtype{#1}\lthtmlvboxmathA}%
\newcommand\lthtmlpictureA{\bgroup\catcode`\_=8 \lthtmlpictureB}%
\newcommand\lthtmlpictureB[1]{\lthtmlmathtype{#1}\egroup
       \let\@savefreelist\@freelist \lthtmlhboxmathB}%
\newcommand\lthtmlpictureZ[1]{\hfill\lthtmlfigureZ}%
\newcommand\lthtmlfigureZ{\lthtmlboxmathZ\lthtmllogmath\copy\sizebox
       \global\let\@freelist\@savefreelist}%
\newcommand\lthtmldisplayA{\bgroup\catcode`\_=8 \lthtmldisplayAi}%
\newcommand\lthtmldisplayAi[1]{\lthtmlmathtype{#1}\egroup\lthtmlvboxmathA}%
\newcommand\lthtmldisplayB[1]{\edef\preveqno{(\theequation)}%
  \lthtmldisplayA{#1}\let\@eqnnum\relax}%
\newcommand\lthtmldisplayZ{\lthtmlboxmathZ\lthtmllogmath\lthtmlsetmath}%
\newcommand\lthtmlinlinemathA{\bgroup\catcode`\_=8 \lthtmlinlinemathB}
\newcommand\lthtmlinlinemathB[1]{\lthtmlmathtype{#1}\egroup\lthtmlhboxmathA
  \vrule height1.5ex width0pt }%
\newcommand\lthtmlinlineA{\bgroup\catcode`\_=8 \lthtmlinlineB}%
\newcommand\lthtmlinlineB[1]{\lthtmlmathtype{#1}\egroup\lthtmlhboxmathA}%
\newcommand\lthtmlinlineZ{\egroup\expandafter\ifdim\dp\sizebox>0pt %
  \expandafter\centerinlinemath\fi\lthtmllogmath\lthtmlsetinline}
\newcommand\lthtmlinlinemathZ{\egroup\expandafter\ifdim\dp\sizebox>0pt %
  \expandafter\centerinlinemath\fi\lthtmllogmath\lthtmlsetmath}
\newcommand\lthtmlindisplaymathZ{\egroup %
  \centerinlinemath\lthtmllogmath\lthtmlsetmath}
\def\lthtmlsetinline{\hbox{\vrule width.1em \vtop{\vbox{%
  \kern.1em\copy\sizebox}\ifdim\dp\sizebox>0pt\kern.1em\else\kern.3pt\fi
  \ifdim\hsize>\wd\sizebox \hrule depth1pt\fi}}}
\def\lthtmlsetmath{\hbox{\vrule width.1em\kern-.05em\vtop{\vbox{%
  \kern.1em\kern0.8 pt\hbox{\hglue.17em\copy\sizebox\hglue0.8 pt}}\kern.3pt%
  \ifdim\dp\sizebox>0pt\kern.1em\fi \kern0.8 pt%
  \ifdim\hsize>\wd\sizebox \hrule depth1pt\fi}}}
\def\centerinlinemath{%
  \dimen1=\ifdim\ht\sizebox<\dp\sizebox \dp\sizebox\else\ht\sizebox\fi
  \advance\dimen1by.5pt \vrule width0pt height\dimen1 depth\dimen1 
 \dp\sizebox=\dimen1\ht\sizebox=\dimen1\relax}

\def\lthtmlcheckvsize{\ifdim\ht\sizebox<\vsize 
  \ifdim\wd\sizebox<\hsize\expandafter\hfill\fi \expandafter\vfill
  \else\expandafter\vss\fi}%
\providecommand{\selectlanguage}[1]{}%
\makeatletter \tracingstats = 1 


\begin{document}
\pagestyle{empty}\thispagestyle{empty}\lthtmltypeout{}%
\lthtmltypeout{latex2htmlLength hsize=\the\hsize}\lthtmltypeout{}%
\lthtmltypeout{latex2htmlLength vsize=\the\vsize}\lthtmltypeout{}%
\lthtmltypeout{latex2htmlLength hoffset=\the\hoffset}\lthtmltypeout{}%
\lthtmltypeout{latex2htmlLength voffset=\the\voffset}\lthtmltypeout{}%
\lthtmltypeout{latex2htmlLength topmargin=\the\topmargin}\lthtmltypeout{}%
\lthtmltypeout{latex2htmlLength topskip=\the\topskip}\lthtmltypeout{}%
\lthtmltypeout{latex2htmlLength headheight=\the\headheight}\lthtmltypeout{}%
\lthtmltypeout{latex2htmlLength headsep=\the\headsep}\lthtmltypeout{}%
\lthtmltypeout{latex2htmlLength parskip=\the\parskip}\lthtmltypeout{}%
\lthtmltypeout{latex2htmlLength oddsidemargin=\the\oddsidemargin}\lthtmltypeout{}%
\makeatletter
\if@twoside\lthtmltypeout{latex2htmlLength evensidemargin=\the\evensidemargin}%
\else\lthtmltypeout{latex2htmlLength evensidemargin=\the\oddsidemargin}\fi%
\lthtmltypeout{}%
\makeatother
\setcounter{page}{1}
\onecolumn

% !!! IMAGES START HERE !!!

{\newpage\clearpage
\lthtmlinlinemathA{tex2html_wrap_inline850}%
$y(x)$%
\lthtmlinlinemathZ
\lthtmlcheckvsize\clearpage}



\selectlanguage{spanish}

\stepcounter{chapter}
\stepcounter{section}
{\newpage\clearpage
\lthtmldisplayA{displaymath391}%
\begin{displaymath}
y^{\prime \prime} + x y=0,
\end{displaymath}%
\lthtmldisplayZ
\lthtmlcheckvsize\clearpage}

\stepcounter{section}
{\newpage\clearpage
\lthtmlinlinemathA{tex2html_wrap_inline441}%
$f$%
\lthtmlinlinemathZ
\lthtmlcheckvsize\clearpage}

{\newpage\clearpage
\lthtmlinlinemathA{tex2html_wrap_inline443}%
$I$%
\lthtmlinlinemathZ
\lthtmlcheckvsize\clearpage}

{\newpage\clearpage
\lthtmlinlinemathA{tex2html_wrap_inline445}%
$f^{\prime}$%
\lthtmlinlinemathZ
\lthtmlcheckvsize\clearpage}

{\newpage\clearpage
\lthtmlinlinemathA{tex2html_wrap_inline447}%
$f^{\prime \prime}$%
\lthtmlinlinemathZ
\lthtmlcheckvsize\clearpage}

{\newpage\clearpage
\lthtmlinlinemathA{tex2html_wrap_inline449}%
$f^{\prime \prime \prime}$%
\lthtmlinlinemathZ
\lthtmlcheckvsize\clearpage}

{\newpage\clearpage
\lthtmldisplayA{eqnarraystar16}%
\begin{eqnarray*}
f(x) & = & a_0 + a_1 x + a_2 x^2 + a_3 x^3 + \ldots = \sum_{i=0}^{\infty} a_n x^n\\
f^{\prime}(x) & = & a_1 + 2 a_2 x + 3 a_3 x^2 + 4 a_4 x^3 + \ldots = \sum_{n=0}^{\infty} n a_n x^{n-1}  \\
f^{\prime \prime}(x) & = & 2 a_2 + 6 a_3 x + 12 a_4 x^2 + 20 a_5 x^3 + \ldots = \sum_{n=0}^{\infty} n \left( n-1 \right) x^{n-2}
\end{eqnarray*}%
\lthtmldisplayZ
\lthtmlcheckvsize\clearpage}

{\newpage\clearpage
\lthtmlinlinemathA{tex2html_wrap_inline451}%
$y^{\prime} - 2y = 0$%
\lthtmlinlinemathZ
\lthtmlcheckvsize\clearpage}

{\newpage\clearpage
\lthtmldisplayA{displaymath392}%
\begin{displaymath}
y = \sum_{n=0}^{\infty} a_n x^n
\end{displaymath}%
\lthtmldisplayZ
\lthtmlcheckvsize\clearpage}

{\newpage\clearpage
\lthtmlinlinemathA{tex2html_wrap_inline453}%
$y^{\prime}$%
\lthtmlinlinemathZ
\lthtmlcheckvsize\clearpage}

{\newpage\clearpage
\lthtmldisplayA{displaymath393}%
\begin{displaymath}
y^{\prime} = \sum_{n=0}^{\infty} n a_n x^{n-1}
\end{displaymath}%
\lthtmldisplayZ
\lthtmlcheckvsize\clearpage}

{\newpage\clearpage
\lthtmldisplayA{eqnarraystar41}%
\begin{eqnarray*}
y^{\prime} - 2y & = & 0 \\
\sum_{n=0}^{\infty} n a_n x^{n-1} - 2 \sum_{n=0}^{\infty} a_n x^n & = & 0 \\
\sum_{n=0}^{\infty} n a_n x^{n-1} & = & 2 \sum_{n=0}^{\infty} a_n x^n \\
\end{eqnarray*}%
\lthtmldisplayZ
\lthtmlcheckvsize\clearpage}

{\newpage\clearpage
\lthtmlinlinemathA{tex2html_wrap_inline455}%
$x^n$%
\lthtmlinlinemathZ
\lthtmlcheckvsize\clearpage}

{\newpage\clearpage
\lthtmldisplayA{displaymath394}%
\begin{displaymath}
\sum_{n=-1}^{\infty} \left(n + 1 \right) a_{n+1} x^n = 2 \sum_{n=0}^{\infty} a_n x^n
\end{displaymath}%
\lthtmldisplayZ
\lthtmlcheckvsize\clearpage}

{\newpage\clearpage
\lthtmldisplayA{displaymath395}%
\begin{displaymath}
\left(n + 1 \right) a_{n+1} = 2 a_n \Rightarrow a_{n+1} = \frac{2a_n}{n+1}
\end{displaymath}%
\lthtmldisplayZ
\lthtmlcheckvsize\clearpage}

{\newpage\clearpage
\lthtmlinlinemathA{tex2html_wrap_inline457}%
$n \geq 0$%
\lthtmlinlinemathZ
\lthtmlcheckvsize\clearpage}

{\newpage\clearpage
\lthtmldisplayA{eqnarraystar63}%
\begin{eqnarray*}
a_1 & = & 2a_0 \\
a_2 & = & \frac{2a_1}{2}=\frac{2^2 a_0}{2} \\
a_3 & = & \frac{2a_2}{3}= \frac{2^3 a_0}{2 \cdot 3}= \frac{2^3 a_0}{3!} \\
a_4 & = & \frac{2a_3}{4} = \frac{2^4 a_0}{2 \cdot 3 \cdot 4} = \frac{2^4 a_0}{4!} \\
\vdots \\
a_n & = & \frac{2^n a_0}{n!} \\
\end{eqnarray*}%
\lthtmldisplayZ
\lthtmlcheckvsize\clearpage}

{\newpage\clearpage
\lthtmldisplayA{displaymath396}%
\begin{displaymath}
y = \sum_{n=0}^{\infty} \frac{2^n a_0}{n!} x^n = a_0 \sum_{n=0}^{\infty} \frac{\left(2 x \right)^n}{n!} = a_0 e^{2x}
\end{displaymath}%
\lthtmldisplayZ
\lthtmlcheckvsize\clearpage}

{\newpage\clearpage
\lthtmldisplayA{displaymath397}%
\begin{displaymath}
e^x = \sum_{n=0}^{\infty} \frac{x^n}{n!}
\end{displaymath}%
\lthtmldisplayZ
\lthtmlcheckvsize\clearpage}

{\newpage\clearpage
\lthtmldisplayA{displaymath398}%
\begin{displaymath}
y^{\prime} - 2 y = 0 \Rightarrow \frac{dy}{y} = 2 dx \Rightarrow Ln(y) = 2x + c  \Rightarrow y = c e^{2x},
\end{displaymath}%
\lthtmldisplayZ
\lthtmlcheckvsize\clearpage}

{\newpage\clearpage
\lthtmlinlinemathA{tex2html_wrap_inline459}%
$y^{\prime \prime} + x y^{\prime} + y = 0$%
\lthtmlinlinemathZ
\lthtmlcheckvsize\clearpage}

{\newpage\clearpage
\lthtmldisplayA{displaymath400}%
\begin{displaymath}
y^{\prime} = \sum_{n=0}^{\infty} n a_n x^{n-1} \Rightarrow xy^{\prime} = \sum_{n=0}^{\infty} n a_n x^n 
\end{displaymath}%
\lthtmldisplayZ
\lthtmlcheckvsize\clearpage}

{\newpage\clearpage
\lthtmldisplayA{displaymath401}%
\begin{displaymath}
y^{\prime \prime} = \sum_{n=0}^{\infty} n \left(n - 1 \right) a_n x^{n-2}
\end{displaymath}%
\lthtmldisplayZ
\lthtmlcheckvsize\clearpage}

{\newpage\clearpage
\lthtmldisplayA{eqnarraystar122}%
\begin{eqnarray*}
\sum_{n=0}^{\infty} n \left( n-1 \right) a_n x^{n-2} + \sum_{n=0}^{\infty} n a_n x^n + \sum_{n=0}^{\infty} a_n x^n & = & 0 \\
\sum_{n=0}^{\infty} n \left( n -1 \right) a_n x^{n-2} & = & -\sum_{n=0}^{\infty} \left(n + 1  \right) a_n x^n \\
\end{eqnarray*}%
\lthtmldisplayZ
\lthtmlcheckvsize\clearpage}

{\newpage\clearpage
\lthtmldisplayA{displaymath402}%
\begin{displaymath}
\sum_{n=-2}^{\infty} \left(n + 2 \right) \left(n + 1 \right) a_{n+2} x^n = - \sum_{n=0}^{\infty} \left(n + 1 \right) a_n x^n
\end{displaymath}%
\lthtmldisplayZ
\lthtmlcheckvsize\clearpage}

{\newpage\clearpage
\lthtmldisplayA{displaymath403}%
\begin{displaymath}
a_{n+2} = - \frac{n + 1}{\left(n+2 \right) \left(n + 1 \right)} a_n = - \frac{a_n}{n+2}
\end{displaymath}%
\lthtmldisplayZ
\lthtmlcheckvsize\clearpage}

{\newpage\clearpage
\lthtmldisplayA{eqnarraystar147}%
\begin{eqnarray*}
a_2 & = & - \frac{a_0}{2} \\
a_4 & = & - \frac{a_2}{4}= \frac{a_0}{2 \cdot 4} \\
a_6 & = & - \frac{a_4}{6} = - \frac{a_0}{2 \cdot 4 \cdot 6} \\
\vdots & & \vdots \\
a_{2n} & = & \frac{(-1)^n a_0}{2 \cdot 4 \cdot 6 \ldots (2n)} = \frac{(-1)^n a_0}{2^n n!}
\end{eqnarray*}%
\lthtmldisplayZ
\lthtmlcheckvsize\clearpage}

{\newpage\clearpage
\lthtmldisplayA{eqnarraystar164}%
\begin{eqnarray*}
a_3 & = & - \frac{a_1}{3} \\
a_5 & = & - \frac{a_3}{5}= \frac{a_1}{3 \cdot 5} \\
a_7 & = & - \frac{a_5}{7} = - \frac{a_1}{3 \cdot 5 \cdot 7} \\
\vdots & & \vdots \\
a_{2n+1} & = & \frac{(-1)^n a_1}{3 \cdot 5 \cdot 7 \ldots (2n+1)}
\end{eqnarray*}%
\lthtmldisplayZ
\lthtmlcheckvsize\clearpage}

{\newpage\clearpage
\lthtmlinlinemathA{tex2html_wrap_inline463}%
$a_0$%
\lthtmlinlinemathZ
\lthtmlcheckvsize\clearpage}

{\newpage\clearpage
\lthtmlinlinemathA{tex2html_wrap_inline465}%
$a_1$%
\lthtmlinlinemathZ
\lthtmlcheckvsize\clearpage}

{\newpage\clearpage
\lthtmldisplayA{displaymath404}%
\begin{displaymath}
y = a_0 \sum_{n=0}^{\infty} \frac{(-1)^n x^{2n}}{2^n n!} + a_1 \sum_{n=0}^{\infty} \frac{(-)^n x^{2n+1}}{3 \cdot 5 \cdot 7 \ldots (2n+1)}
\end{displaymath}%
\lthtmldisplayZ
\lthtmlcheckvsize\clearpage}

{\newpage\clearpage
\lthtmlinlinemathA{tex2html_wrap_inline473}%
$n+1$%
\lthtmlinlinemathZ
\lthtmlcheckvsize\clearpage}

{\newpage\clearpage
\lthtmlinlinemathA{tex2html_wrap_inline477}%
$c$%
\lthtmlinlinemathZ
\lthtmlcheckvsize\clearpage}

{\newpage\clearpage
\lthtmlinlinemathA{tex2html_wrap_inline479}%
$x$%
\lthtmlinlinemathZ
\lthtmlcheckvsize\clearpage}

{\newpage\clearpage
\lthtmlinlinemathA{tex2html_wrap_inline483}%
$z$%
\lthtmlinlinemathZ
\lthtmlcheckvsize\clearpage}

{\newpage\clearpage
\lthtmlinlinemathA{tex2html_wrap_inline485}%
$a$%
\lthtmlinlinemathZ
\lthtmlcheckvsize\clearpage}

{\newpage\clearpage
\lthtmldisplayA{displaymath405}%
\begin{displaymath}
f(x) = \sum_{n=0}^n \frac{f^{(n)}(c)}{n!} \left(x - c \right)^n + \frac{f^{(n+1)} \left(z \right)}{(n+1)!} \left( x - c  \right)^{n+1}
\end{displaymath}%
\lthtmldisplayZ
\lthtmlcheckvsize\clearpage}

{\newpage\clearpage
\lthtmldisplayA{displaymath406}%
\begin{displaymath}
\left\{
\begin{array}{rcl}
y^{\prime} & = & y^2 -x \\
y(0) & = & 1
\end{array}
\right.
\end{displaymath}%
\lthtmldisplayZ
\lthtmlcheckvsize\clearpage}

{\newpage\clearpage
\lthtmlinlinemathA{tex2html_wrap_inline489}%
$y$%
\lthtmlinlinemathZ
\lthtmlcheckvsize\clearpage}

{\newpage\clearpage
\lthtmlinlinemathA{tex2html_wrap_inline491}%
$[0,1]$%
\lthtmlinlinemathZ
\lthtmlcheckvsize\clearpage}

{\newpage\clearpage
\lthtmlinlinemathA{tex2html_wrap_inline493}%
$0.1$%
\lthtmlinlinemathZ
\lthtmlcheckvsize\clearpage}

{\newpage\clearpage
\lthtmldisplayA{displaymath407}%
\begin{displaymath}
y = y(0) + \frac{y^{\prime}(0)}{1!} x + \frac{y^{\prime \prime}(0)}{2!} x^2  + \frac{y^{\prime \prime}(0)}{3!} x^3 + \ldots
\end{displaymath}%
\lthtmldisplayZ
\lthtmlcheckvsize\clearpage}

{\newpage\clearpage
\lthtmlinlinemathA{tex2html_wrap_inline497}%
$c=0$%
\lthtmlinlinemathZ
\lthtmlcheckvsize\clearpage}

{\newpage\clearpage
\lthtmlinlinemathA{tex2html_wrap_inline499}%
$y(0)=1$%
\lthtmlinlinemathZ
\lthtmlcheckvsize\clearpage}

{\newpage\clearpage
\lthtmlinlinemathA{tex2html_wrap_inline501}%
$y^{\prime} = y^2 - x$%
\lthtmlinlinemathZ
\lthtmlcheckvsize\clearpage}

{\newpage\clearpage
\lthtmldisplayA{eqnarraystar212}%
\begin{eqnarray*}
y^{\prime} = y^2 -x & \Rightarrow & y^{\prime}(0) = 1 \\
y^{\prime \prime} = 2yy^{\prime} - 1 & \Rightarrow & y^{\prime \prime}(0) = 2-1=1  \\
y^{\prime \prime \prime} = 2yy^{\prime \prime} + 2 \left( y^{\prime} \right)^2 & \Rightarrow & y^{\prime \prime \prime}(0)=2+2=4 \\
y^{(4)} = 2yy^{\prime \prime \prime} + 6y^{\prime}y^{\prime \prime} &  \Rightarrow & y^{(4)} = 8 + 6 = 14 \\
y^{(5)} = 2yy^{(4)} + 8y^{\prime} y^{\prime \prime \prime} + 6 \left( y^{\prime \prime} \right)^2 & \Rightarrow & y^{(5)}(0) = 28 + 32 + 6 = 66 \\
\end{eqnarray*}%
\lthtmldisplayZ
\lthtmlcheckvsize\clearpage}

{\newpage\clearpage
\lthtmldisplayA{displaymath408}%
\begin{displaymath}
y = 1 + x + \frac{1}{2} x^2 + \frac{4}{3!} x^3 + \frac{14}{4!} x^4 + \frac{66}{5!} x^5 + \ldots
\end{displaymath}%
\lthtmldisplayZ
\lthtmlcheckvsize\clearpage}

{\newpage\clearpage
\lthtmlinlinemathA{tex2html_wrap_inline515}%
$x=a$%
\lthtmlinlinemathZ
\lthtmlcheckvsize\clearpage}

{\newpage\clearpage
\lthtmlinlinemathA{tex2html_wrap_inline519}%
$c=a$%
\lthtmlinlinemathZ
\lthtmlcheckvsize\clearpage}

{\newpage\clearpage
\lthtmlpictureA{tex2html_wrap952}%
\includegraphics{serie1.eps}%
\lthtmlpictureZ
\lthtmlcheckvsize\clearpage}

{\newpage\clearpage
\lthtmldisplayA{displaymath409}%
\begin{displaymath}
y^{\prime \prime} + Sen(x) y^{\prime} + e^x y = 0
\end{displaymath}%
\lthtmldisplayZ
\lthtmlcheckvsize\clearpage}

{\newpage\clearpage
\lthtmlinlinemathA{tex2html_wrap_inline523}%
$x=0$%
\lthtmlinlinemathZ
\lthtmlcheckvsize\clearpage}

{\newpage\clearpage
\lthtmldisplayA{displaymath410}%
\begin{displaymath}
y = a_0 + a_1x + a_2x^2 + a_3x^3 + \ldots + a_n x^n + \ldots = \sum_{n=0}^{\infty} a_n x^n
\end{displaymath}%
\lthtmldisplayZ
\lthtmlcheckvsize\clearpage}

{\newpage\clearpage
\lthtmldisplayA{displaymath411}%
\begin{displaymath}
Sen(x) = x - \frac{1}{3!} x^3 + \frac{1}{5!} x^5 + \ldots + \frac{(-1)^n}{(2n+1)!} x^{2n+1}  = \sum_{n=0}^{\infty} \frac{(-1)^n}{(2n+1)!} x^{2n+1}
\end{displaymath}%
\lthtmldisplayZ
\lthtmlcheckvsize\clearpage}

{\newpage\clearpage
\lthtmldisplayA{displaymath412}%
\begin{displaymath}
e^x = 1 +x + \frac{1}{2!} x^2 + \frac{1}{3!} x^3 + \ldots + \frac{1}{n!} x^n + \ldots = \sum_{n=0}^{\infty} \frac{1}{n!}x^n
\end{displaymath}%
\lthtmldisplayZ
\lthtmlcheckvsize\clearpage}

{\newpage\clearpage
\lthtmlinlinemathA{tex2html_wrap_inline529}%
$x \in  \mbox{$I \hspace{-1.3mm} R$} $%
\lthtmlinlinemathZ
\lthtmlcheckvsize\clearpage}

{\newpage\clearpage
\lthtmldisplayA{eqnarraystar287}%
\begin{eqnarray*}
\sum_{n=0}^{\infty} n\left( n-1 \right)a_n x^{n-2} + \left( \sum_{n=0}^{\infty} \frac{(-1)^n}{(2n+1)!} x^{2n+1}  \right) \left( \sum_{n=0}^{\infty} n a_n x^{n-1}\right) & + & \\
 \left(  \sum_{n=0}^{\infty} \frac{1}{n!}x^n \right) \left( \sum_{n=0}^{\infty} a_n x^n  \right) & = & 0
\end{eqnarray*}%
\lthtmldisplayZ
\lthtmlcheckvsize\clearpage}

{\newpage\clearpage
\lthtmldisplayA{eqnarraystar306}%
\begin{eqnarray*}
\left(2a_2 + a_0  \right) + \left(6a_3 + 2a_1 + a_0 \right)x + \left(12a_4 + 3a_2 + a_1 + \frac{a_0}{2}  \right)x^2 & + & \\
\left(20a_5 + 4a_3 + a_2 + \frac{a_1}{2} + \frac{a_0}{6} \right) x^3 + \ldots & = & 0
\end{eqnarray*}%
\lthtmldisplayZ
\lthtmlcheckvsize\clearpage}

{\newpage\clearpage
\lthtmldisplayA{eqnarraystar314}%
\begin{eqnarray*}
a_2 & = & - \frac{a_0}{2} \\
a_3 & = & - \frac{2a_1 + a_0}{6}=- \frac{a_1}{3} - \frac{a_0}{6} \\
a_4 & = & - \frac{a_2}{4} - \frac{a_1}{12} - \frac{a_0}{24} = \frac{a_0}{8} - \frac{a_1}{12} - \frac{a_0}{24} = \frac{a_0}{12} - \frac{a_1}{12} \\
a_5 & = & - \frac{a_3}{5} - \frac{a_2}{20} - \frac{a_1}{60} - \frac{a_0}{120} = \frac{a_0}{20} + \frac{a_1}{20}
\end{eqnarray*}%
\lthtmldisplayZ
\lthtmlcheckvsize\clearpage}

{\newpage\clearpage
\lthtmldisplayA{displaymath413}%
\begin{displaymath}
y = a_0 \left(1 - \frac{1}{2} x^2 - \frac{1}{6} x^3 + \frac{1}{12} x^4 + \frac{1}{20} x^5 + \ldots   \right) + a_1 \left(   x - \frac{1}{3} x^3 - \frac{1}{12} x^4 + \frac{1}{20} x^5 + \ldots \right)
\end{displaymath}%
\lthtmldisplayZ
\lthtmlcheckvsize\clearpage}

{\newpage\clearpage
\lthtmldisplayA{displaymath414}%
\begin{displaymath}
\left( \sum_{n=0}^{\infty} a_n x^n \right) \left( \sum_{n=0}^{\infty} b_n x^n  \right) = \sum_{n=0}^{\infty} \left( \sum_{k=0}^{n} a_k b_{n-k}\right) x^n
\end{displaymath}%
\lthtmldisplayZ
\lthtmlcheckvsize\clearpage}


\end{document}
